@prefix : <http://purl.oclc.org/NET/ldr/ns#> .
@prefix cc: <http://creativecommons.org/ns#> .
@prefix dc: <http://purl.org/dc/elements/1.1/> .
@prefix acl: <http://www.w3.org/ns/auth/acl#> .
@prefix dct: <http://purl.org/dc/terms/> .
@prefix ldp: <http://www.w3.org/ns/ldp#> .
@prefix owl: <http://www.w3.org/2002/07/owl#> .
@prefix rdf: <http://www.w3.org/1999/02/22-rdf-syntax-ns#> .
@prefix xml: <http://www.w3.org/XML/1998/namespace> .
@prefix xsd: <http://www.w3.org/2001/XMLSchema#> .
@prefix foaf: <http://xmlns.com/foaf/0.1/> .
@prefix frbr: <http://purl.org/vocab/frbr/core#> .
@prefix lkif: <http://www.estrellaproject.org/lkif-core/lkif-core.owl> .
@prefix odrl: <http://www.w3.org/ns/odrl/2/> .
@prefix prov: <http://www.w3.org/ns/prov#> .
@prefix rdfs: <http://www.w3.org/2000/01/rdf-schema#> .
@prefix skos: <http://www.w3.org/2004/02/skos/core#> .
@prefix vann: <http://purl.org/vocab/vann/> .
@prefix voaf: <http://purl.org/vocommons/voaf#> .
@prefix void: <http://rdfs.org/ns/void#> .
@prefix mco-core: <urn:mpeg:mpeg21:mco:core:2012#> .
@prefix cpannotationschema: <http://www.ontologydesignpatterns.org/schemas/cpannotationschema.owl#> .
@base <http://purl.oclc.org/NET/ldr/ns#> .

<http://purl.oclc.org/NET/ldr/ns#> rdf:type owl:Ontology ;
                                   
                                   rdfs:label "Linked Data Rights"@en ;
                                   
                                   voaf:propertyNumber "18"^^xsd:int ;
                                   
                                   dct:issued "2013-09-20"^^xsd:date ,
                                              "2014-08-30"^^xsd:date ;
                                   
                                   voaf:classNumber "31"^^xsd:int ;
                                   
                                   cpannotationschema:scenarios "Declaring rights on both Linked Open Data and Linked Closed Data"@en ;
                                   
                                   dct:title "Linked Data Rights (LDR)"@en ;
                                   
                                   dct:contributor "Maria Poveda-Villalon" ;
                                   
                                   vann:preferredNamespacePrefix "ldr" ;
                                   
                                   dct:contributor "Asuncion Gomez-Perez" ,
                                                   "Victor Rodriguez-Doncel" ;
                                   
                                   owl:versionInfo "2.0"@en ;
                                   
                                   dct:creator "Ontology Engineering Group - Universidad Polit√©cnica de Madrid" ;
                                   
                                   dct:description """The Linked Data Rights ontology provides the vocabulary for creating rights expressions for Linked Data resources by extending the ODRL ontology. 
								   Linked Data assets (RDF triples, graphs, datasets, mappings...) can be object of protection by the intellectual property law, the database law or its access or publication be restricted by other legal reasons (personal data pro- tection, security reasons, etc.). Publishing a rights expression along with the digital asset, allows the rightsholder waiving some or all of the IP and database rights (leaving the work in the public domain), permitting some operations if certain conditions are satisfied (like giving attribution to the author) or simply reminding the audience that some rights are reserved. Specific vocabulary is given for authorising specific uses of Linked Data."""@en ;
                                   
                                   vann:preferredNamespaceUri "http://purl.oclc.org/NET/ldr/ns#" ;
                                   
                                   dct:contributor "Mari Carmen Suarez" ;
                                   
                                   cpannotationschema:hasComponent "http://www.w3.org/TR/swbp-n-aryRelations/"@en ;
                                   
                                   cc:license <http://creativecommons.org/licenses/by/3.0/> ;
                                   
                                   voaf:hasEquivalencesWith cc:null ;
                                   
                                   voaf:specializes cc:null ;
                                   
                                   voaf:reliesOn cc:null ;
                                   
                                   voaf:similar <http://data.opendataday.it/LiMo> ;
                                   
                                   dc:creator <http://delicias.dia.fi.upm.es/~vrodriguez/> ;
                                   
                                   voaf:similar <http://ns.inria.fr/l4lod/v2/l4lod_v2.rdf> ;
                                   
                                   cpannotationschema:hasIntent <http://oeg-dev.dia.fi.upm.es/licensius/static/ldr/pattern.html#int> ;
                                   
                                   cpannotationschema:coversRequirements <http://oeg-dev.dia.fi.upm.es/licensius/static/ldr/pattern.html#reqs> ;
                                   
                                   prov:wasDerivedFrom <http://oeg-dev.dia.fi.upm.es/licensius/static/lldr/lldr-2013.07.18.owl> ;
                                   
                                   voaf:similar <http://schema.theodi.org/odrs/> ;
                                   
                                   voaf:reliesOn odrl: ;
                                   
                                   voaf:similar odrl:null ;
                                   
                                   voaf:reliesOn odrl:null ;
                                   
                                   voaf:specializes odrl:null ;
                                   
                                   voaf:hasEquivalencesWith odrl:null ,
                                                            foaf:null .


#################################################################
#
#    Annotation properties
#
#################################################################


###  http://purl.oclc.org/NET/ldr/ns#issuedOn

:issuedOn rdf:type owl:AnnotationProperty ;
          
          rdfs:comment "Date on which the rights expression is issued, with legal consequences on the copyright or database right expiration."@en ;
          
          rdfs:domain :Policy .



###  http://www.w3.org/2004/02/skos/core#closeMatch

skos:closeMatch rdf:type owl:AnnotationProperty .



###  http://www.w3.org/2004/02/skos/core#exactMatch

skos:exactMatch rdf:type owl:AnnotationProperty .



###  http://www.w3.org/2004/02/skos/core#example

skos:example rdf:type owl:AnnotationProperty .



###  http://www.w3.org/2004/02/skos/core#narrowMatch

skos:narrowMatch rdf:type owl:AnnotationProperty .





#################################################################
#
#    Object Properties
#
#################################################################


###  http://purl.oclc.org/NET/ldr/ns#hasClaim

:hasClaim rdf:type owl:ObjectProperty ;
          
          rdfs:comment "Declares a claim asserted in the context of a rights expression"@en ;
          
          rdfs:range :Proposition .



###  http://purl.oclc.org/NET/ldr/ns#hasExtendedRule

:hasExtendedRule rdf:type owl:ObjectProperty ;
                 
                 rdfs:comment "Links a Policy to an ExtendedRule it contains"@en ;
                 
                 rdfs:range :ExtendedRule ;
                 
                 rdfs:domain odrl:Policy .



###  http://purl.oclc.org/NET/ldr/ns#hasLegalStatus

:hasLegalStatus rdf:type owl:ObjectProperty ;
                
                rdfs:comment "Declares the legal status of a resource" ;
                
                rdfs:domain :LinkedDataResource ;
                
                rdfs:range :ResourceLegalStatus .



###  http://purl.oclc.org/NET/ldr/ns#hasRequirement

:hasRequirement rdf:type owl:ObjectProperty ;
                
                rdfs:comment "Declares which requirements have to be fulfilled for the Rule to be valid"@en ;
                
                rdfs:range :Proposition ;
                
                rdfs:domain odrl:Rule .





#################################################################
#
#    Data properties
#
#################################################################


###  http://purl.oclc.org/NET/ldr/ns#dataFormat

:dataFormat rdf:type owl:DatatypeProperty ;
            
            rdfs:comment "Format of the data (\"text/html\", \"application/rdf+xml\", etc.)"@en ;
            
            rdfs:subPropertyOf :hasclaim ,
                               odrl:rightOperand .



###  http://purl.oclc.org/NET/ldr/ns#hasAttributionText

:hasAttributionText rdf:type owl:DatatypeProperty ;
                    
                    rdfs:comment "Text that has to be included as requested by a condition"@en ;
                    
                    skos:closeMatch cc:attributionName ,
                                    cc:attributionURL ;
                    
                    rdfs:domain :Proposition ;
                    
                    rdfs:subPropertyOf :hasclaim ;
                    
                    rdfs:range rdfs:Literal ;
                    
                    rdfs:subPropertyOf odrl:rightOperand .



###  http://purl.oclc.org/NET/ldr/ns#hasCopyrightNotice

:hasCopyrightNotice rdf:type owl:DatatypeProperty ;
                    
                    rdfs:comment "Text that has to be attached imposed as a condition"@en ;
                    
                    rdfs:subPropertyOf :hasclaim ;
                    
                    rdfs:range rdfs:Literal ;
                    
                    rdfs:subPropertyOf odrl:rightOperand .



###  http://purl.oclc.org/NET/ldr/ns#hasDisclaimerText

:hasDisclaimerText rdf:type owl:DatatypeProperty ;
                   
                   rdfs:comment "Text discharging responsibilities on the use of the Linked Data resource"@en ;
                   
                   rdfs:subPropertyOf :hasclaim ;
                   
                   rdfs:domain odrl:Policy ;
                   
                   rdfs:subPropertyOf odrl:rightOperand .



###  http://purl.oclc.org/NET/ldr/ns#hasPersonalData

:hasPersonalData rdf:type owl:DatatypeProperty ;
                 
                 rdfs:comment "Declares that the referred resource has personal data"@en ;
                 
                 rdfs:subPropertyOf :hasclaim ,
                                    odrl:rightOperand .



###  http://purl.oclc.org/NET/ldr/ns#hasPrivacyLevel

:hasPrivacyLevel rdf:type owl:DatatypeProperty ;
                 
                 rdfs:comment "Declares the privacy level (e.g. personal data) for a Linked Data resource"@en ;
                 
                 rdfs:domain :LinkedDataResource ;
                 
                 rdfs:subPropertyOf :hasclaim ,
                                    odrl:rightOperand .



###  http://purl.oclc.org/NET/ldr/ns#hasclaim

:hasclaim rdf:type owl:DatatypeProperty .



###  http://purl.oclc.org/NET/ldr/ns#issuedOn

:issuedOn rdf:type owl:DatatypeProperty ;
          
          rdfs:comment "Date on which the rights expression is issued, with legal consequences on the copyright or database right expiration."@en ;
          
          rdfs:range xsd:dateTime .



###  http://purl.oclc.org/NET/ldr/ns#operation

:operation rdf:type owl:DatatypeProperty ;
           
           rdfs:comment "May be set with one of the mathematical values AND, OR and XOR. (OR is the default if not specified.)"@en ;
           
           rdfs:domain :ExtendedRule ;
           
           rdfs:range xsd:string .



###  http://purl.oclc.org/NET/ldr/ns#protocol

:protocol rdf:type owl:DatatypeProperty ;
          
          rdfs:comment "Access protocol (e.g. \"SPARQL\", \"HTTPS\", etc.)"@en ;
          
          rdfs:subPropertyOf :hasclaim ,
                             odrl:rightOperand .



###  http://purl.oclc.org/NET/ldr/ns#queriesPerDay

:queriesPerDay rdf:type owl:DatatypeProperty ;
               
               rdfs:comment "Number of queries per day"@en ;
               
               rdfs:subPropertyOf :hasclaim ,
                                  odrl:rightOperand .



###  http://purl.oclc.org/NET/ldr/ns#queriesPerMinute

:queriesPerMinute rdf:type owl:DatatypeProperty ;
                  
                  rdfs:comment "Number of queries per minute"@en ;
                  
                  rdfs:subPropertyOf :hasclaim ,
                                     odrl:rightOperand .



###  http://purl.oclc.org/NET/ldr/ns#truthValue

:truthValue rdf:type owl:DatatypeProperty ;
            
            rdfs:comment "Truth value"@en ;
            
            rdfs:domain :Proposition ;
            
            rdfs:range xsd:boolean .



###  http://www.w3.org/ns/odrl/2/rightOperand

odrl:rightOperand rdf:type owl:DatatypeProperty .





#################################################################
#
#    Classes
#
#################################################################


###  http://purl.oclc.org/NET/ldr/ns#Access

:Access rdf:type owl:Class ;
        
        rdfs:subClassOf :LinkedDataRight ;
        
        rdfs:comment "Right of access, which can be legally granted (e.g. public sector information) or expressely restricted (e.g. secrets compromising national security)"@en ;
        
        skos:exactMatch acl:Access .



###  http://purl.oclc.org/NET/ldr/ns#Action

:Action rdf:type owl:Class .



###  http://purl.oclc.org/NET/ldr/ns#CopyrightException

:CopyrightException rdf:type owl:Class ;
                    
                    rdfs:subClassOf :Proposition ;
                    
                    rdfs:comment "Reason which can be invoked to make an exception to the intellectual property or database law "@en .



###  http://purl.oclc.org/NET/ldr/ns#DatabaseRight

:DatabaseRight rdf:type owl:Class ;
               
               rdfs:subClassOf :LinkedDataRight ;
               
               rdfs:comment "Sui generis right for databases, recognized in European countries and others"@en .



###  http://purl.oclc.org/NET/ldr/ns#Derivation

:Derivation rdf:type owl:Class ;
            
            rdfs:subClassOf :IPRight ;
            
            rdfs:comment "Transformation of the work, including translation adaptation or any other form modification"@en ;
            
            skos:closeMatch cc:DerivativeWorks .



###  http://purl.oclc.org/NET/ldr/ns#Distribution

:Distribution rdf:type owl:Class ;
              
              rdfs:subClassOf :IPRight ;
              
              rdfs:comment "Make available the original work or its copies, in a physical medium"@en ;
              
              skos:exactMatch cc:Distribution .



###  http://purl.oclc.org/NET/ldr/ns#ExtendedRule

:ExtendedRule rdf:type owl:Class ;
              
              rdfs:subClassOf odrl:Rule ;
              
              rdfs:comment "Extended Relations may tie Permission, Prohibition, Duty, and Constraint entities together with an AND, OR or XOR relationship. Only entities of the same type can be linked with this model. For example, a Permission and Prohibition cannot be linked together within this model. The Extended rule is composed of two or more rules" .



###  http://purl.oclc.org/NET/ldr/ns#Extraction

:Extraction rdf:type owl:Class ;
            
            rdfs:subClassOf :DatabaseRight ;
            
            rdfs:comment "Right to permanent or temporary transfer of all or a substantial part of the contents of a database to another medium by any means or in any form"@en .



###  http://purl.oclc.org/NET/ldr/ns#FamousDataLicense

:FamousDataLicense rdf:type owl:Class ;
                   
                   rdfs:subClassOf :License ;
                   
                   rdfs:comment "License publicly available and known to the public"@en .



###  http://purl.oclc.org/NET/ldr/ns#IPRight

:IPRight rdf:type owl:Class ;
         
         rdfs:subClassOf :LinkedDataRight ;
         
         rdfs:comment "Intellectual Property right"@en .



###  http://purl.oclc.org/NET/ldr/ns#LDPAccess

:LDPAccess rdf:type owl:Class ;
           
           rdfs:subClassOf :Access .



###  http://purl.oclc.org/NET/ldr/ns#License

:License rdf:type owl:Class ;
         
         rdfs:subClassOf :LinkedDataPolicy ;
         
         rdfs:comment "Set of rights expressions offered to the public, which grant one or more rights, possibly conditioned to the fulfillment of one or more conditions (propositions)"@en .



###  http://purl.oclc.org/NET/ldr/ns#LinkedDataPolicy

:LinkedDataPolicy rdf:type owl:Class ;
                  
                  rdfs:subClassOf odrl:Policy ;
                  
                  rdfs:comment "A policy applied over a Linked Data resource"@en .



###  http://purl.oclc.org/NET/ldr/ns#LinkedDataResource

:LinkedDataResource rdf:type owl:Class ;
                    
                    rdfs:subClassOf odrl:Asset ;
                    
                    rdfs:comment "A Linked Data resource, object of some rights"@en .



###  http://purl.oclc.org/NET/ldr/ns#LinkedDataRight

:LinkedDataRight rdf:type owl:Class ;
                 
                 rdfs:subClassOf :Action ;
                 
                 rdfs:comment "Action legally granted as allowable to be exercised on a Linked Data resource"@en .



###  http://purl.oclc.org/NET/ldr/ns#Proposition

:Proposition rdf:type owl:Class ;
             
             rdfs:comment "A veritative statement"@en .



###  http://purl.oclc.org/NET/ldr/ns#PublicCommunication

:PublicCommunication rdf:type owl:Class ;
                     
                     rdfs:subClassOf :IPRight ;
                     
                     rdfs:comment "Granting a number of people access to the work without existing distribution"@en .



###  http://purl.oclc.org/NET/ldr/ns#Reproduction

:Reproduction rdf:type owl:Class ;
              
              rdfs:subClassOf :IPRight ;
              
              rdfs:comment "Direct or indirect fixation, allowing its communication and/or making copies of it"@en ;
              
              skos:exactMatch cc:Reproduction .



###  http://purl.oclc.org/NET/ldr/ns#ResourceLegalStatus

:ResourceLegalStatus rdf:type owl:Class ;
                     
                     rdfs:subClassOf :Proposition ;
                     
                     rdfs:comment "Attribute of a resource regarding its legal status"@en .



###  http://purl.oclc.org/NET/ldr/ns#Reutilization

:Reutilization rdf:type owl:Class ;
               
               rdfs:subClassOf :DatabaseRight ;
               
               rdfs:comment "Right to make available to the public all or a substantial part of the contents of a database by the distribution of copies, by renting, by on-line or other forms of transmission"@en .



###  http://purl.oclc.org/NET/ldr/ns#SPARQLAccess

:SPARQLAccess rdf:type owl:Class ;
              
              rdfs:subClassOf :Access .



###  http://rdfs.org/ns/void#Dataset

void:Dataset rdf:type owl:Class ;
             
             rdfs:subClassOf :LinkedDataResource .



###  http://rdfs.org/ns/void#Linkset

void:Linkset rdf:type owl:Class ;
             
             rdfs:subClassOf :LinkedDataResource .



###  http://www.w3.org/1999/02/22-rdf-syntax-ns#Statement

rdf:Statement rdf:type owl:Class ;
              
              rdfs:subClassOf :LinkedDataResource .



###  http://www.w3.org/2002/07/owl#Ontology

owl:Ontology rdf:type owl:Class ;
             
             rdfs:subClassOf :LinkedDataResource .



###  http://www.w3.org/ns/ldp#Resource

ldp:Resource rdf:type owl:Class ;
             
             rdfs:subClassOf :LinkedDataResource .



###  http://www.w3.org/ns/odrl/2/Asset

odrl:Asset rdf:type owl:Class .



###  http://www.w3.org/ns/odrl/2/Constraint

odrl:Constraint rdf:type owl:Class ;
                
                rdfs:subClassOf :Proposition .



###  http://www.w3.org/ns/odrl/2/Policy

odrl:Policy rdf:type owl:Class .



###  http://www.w3.org/ns/odrl/2/Rule

odrl:Rule rdf:type owl:Class .



###  urn:mpeg:mpeg21:mco:core:2012#Contract

mco-core:Contract rdf:type owl:Class ;
                  
                  rdfs:subClassOf :LinkedDataPolicy .





#################################################################
#
#    Individuals
#
#################################################################


###  http://purl.oclc.org/NET/ldr/ns#HTTPDELETE

:HTTPDELETE rdf:type :LDPAccess ,
                     owl:NamedIndividual ;
            
            rdfs:comment "Accessing with the HTTP DELETE Method"@en .



###  http://purl.oclc.org/NET/ldr/ns#HTTPGET

:HTTPGET rdf:type :LDPAccess ,
                  owl:NamedIndividual ;
         
         rdfs:comment "Accessing with the HTTP GET Method"@en .



###  http://purl.oclc.org/NET/ldr/ns#HTTPPATCH

:HTTPPATCH rdf:type :LDPAccess ,
                    owl:NamedIndividual ;
           
           rdfs:comment "Accesing with the HTTP PATH Method"@en .



###  http://purl.oclc.org/NET/ldr/ns#HTTPPOST

:HTTPPOST rdf:type :LDPAccess ,
                   owl:NamedIndividual ;
          
          rdfs:comment "Accessing with the HTTP POST Method"@en .



###  http://purl.oclc.org/NET/ldr/ns#HTTPPUT

:HTTPPUT rdf:type :LDPAccess ,
                  owl:NamedIndividual ;
         
         rdfs:comment "Accessing with the HTTP PUT Method"@en .



###  http://purl.oclc.org/NET/ldr/ns#LinkedDataAccess

:LinkedDataAccess rdf:type :Access ,
                           owl:NamedIndividual ;
                  
                  rdfs:label "Retrieval of Linked Data resources"@en .



###  http://purl.oclc.org/NET/ldr/ns#SPARQLASK

:SPARQLASK rdf:type :SPARQLAccess ,
                    owl:NamedIndividual ;
           
           rdfs:comment "Access through the SPARQL ASK query form"@en .



###  http://purl.oclc.org/NET/ldr/ns#SPARQLCONSTRUCT

:SPARQLCONSTRUCT rdf:type :SPARQLAccess ,
                          owl:NamedIndividual ;
                 
                 rdfs:comment "Access through the SPARQL CONSTRUCT query form"@en .



###  http://purl.oclc.org/NET/ldr/ns#SPARQLDESCRIBE

:SPARQLDESCRIBE rdf:type :SPARQLAccess ,
                         owl:NamedIndividual ;
                
                rdfs:comment "Access through the SPARQL DESCRIBE query form"@en .



###  http://purl.oclc.org/NET/ldr/ns#SPARQLSELECT

:SPARQLSELECT rdf:type :SPARQLAccess ,
                       owl:NamedIndividual ;
              
              rdfs:comment "Access through the SPARQL SELECT query form"@en .



###  http://purl.oclc.org/NET/ldr/ns#access

:access rdf:type :Access ,
                 owl:NamedIndividual ;
        
        rdfs:comment "Access in any manner or form" .



###  http://purl.oclc.org/NET/ldr/ns#baseSoftwareUpon

:baseSoftwareUpon rdf:type :Distribution ,
                           owl:NamedIndividual ;
                  
                  rdfs:comment "Distribute a pice of software whose well functioning depends on the related Linked Data resource"@en .



###  http://purl.oclc.org/NET/ldr/ns#copyDatabase

:copyDatabase rdf:type :Extraction ,
                       owl:NamedIndividual ;
              
              rdfs:comment "Coyping a dataset, for other purposes than private use"@en .



###  http://purl.oclc.org/NET/ldr/ns#copyWork

:copyWork rdf:type :Reproduction ,
                   owl:NamedIndividual ;
          
          rdfs:comment "copying the work for purposes other than private"@en .



###  http://purl.oclc.org/NET/ldr/ns#derivation

:derivation rdf:type :Derivation ,
                     owl:NamedIndividual ;
            
            rdfs:comment "General transformation of the work"@en .



###  http://purl.oclc.org/NET/ldr/ns#deriveClasses

:deriveClasses rdf:type :Derivation ,
                        owl:NamedIndividual ;
               
               rdfs:comment "Subclassing"@en .



###  http://purl.oclc.org/NET/ldr/ns#deriveProperties

:deriveProperties rdf:type :Derivation ,
                           owl:NamedIndividual ;
                  
                  rdfs:comment "Subpropertying"@en .



###  http://purl.oclc.org/NET/ldr/ns#distribution

:distribution rdf:type :Distribution ,
                       owl:NamedIndividual ;
              
              rdfs:comment "General act of making available the original work or its copies, in a physical medium"@en .



###  http://purl.oclc.org/NET/ldr/ns#downloadDatabase

:downloadDatabase rdf:type :Extraction ,
                           owl:NamedIndividual ;
                  
                  rdfs:comment "Downloading a dataset, for other purposes than private use"@en .



###  http://purl.oclc.org/NET/ldr/ns#downloadWork

:downloadWork rdf:type :Reproduction ,
                       owl:NamedIndividual ;
              
              rdfs:comment "downloading the work for purposes other than private"@en .



###  http://purl.oclc.org/NET/ldr/ns#extract

:extract rdf:type :Extraction ,
                  owl:NamedIndividual ;
         
         rdfs:comment "General right of extraction"@en .



###  http://purl.oclc.org/NET/ldr/ns#hasAllRightsReserved

:hasAllRightsReserved rdf:type :ResourceLegalStatus ,
                               owl:NamedIndividual ;
                      
                      rdfs:comment "Declares that the referred resource is protected under copyright or database rights, and none of them is waived"@en .



###  http://purl.oclc.org/NET/ldr/ns#hasCopyrightExpired

:hasCopyrightExpired rdf:type :ResourceLegalStatus ,
                              owl:NamedIndividual ;
                     
                     rdfs:comment "Declares that the referred resource has its copyright expired"@en .



###  http://purl.oclc.org/NET/ldr/ns#hasDatabaseRightsExpired

:hasDatabaseRightsExpired rdf:type :ResourceLegalStatus ,
                                   owl:NamedIndividual ;
                          
                          rdfs:comment "Declares that the referred resource has the database rights expired"@en .



###  http://purl.oclc.org/NET/ldr/ns#hasIndustrialSecret

:hasIndustrialSecret rdf:type :ResourceLegalStatus ,
                              owl:NamedIndividual ;
                     
                     rdfs:comment "The referred resource containts an Industrial Secret"@en .



###  http://purl.oclc.org/NET/ldr/ns#hasNationalSecurityInfo

:hasNationalSecurityInfo rdf:type :ResourceLegalStatus ,
                                  owl:NamedIndividual ;
                         
                         rdfs:comment "Declares that the referred resource has information whose disclosure might harm the national security"@en .



###  http://purl.oclc.org/NET/ldr/ns#hasPersonalData

:hasPersonalData rdf:type :ResourceLegalStatus ,
                          owl:NamedIndividual ;
                 
                 rdfs:comment "Declares that the referred resource has personal data"@en .



###  http://purl.oclc.org/NET/ldr/ns#hasTopSecret

:hasTopSecret rdf:type :ResourceLegalStatus ,
                       owl:NamedIndividual ;
              
              rdfs:comment "Declares that the referred resource contains top secret information of military nature or other"@en .



###  http://purl.oclc.org/NET/ldr/ns#isInPublicDomain

:isInPublicDomain rdf:type :ResourceLegalStatus ,
                           owl:NamedIndividual ;
                  
                  rdfs:comment "Declares that the declared resource is in the public domain"@en .



###  http://purl.oclc.org/NET/ldr/ns#judicialProcess

:judicialProcess rdf:type :CopyrightException ,
                          owl:NamedIndividual ;
                 
                 rdfs:comment "if the action is carried out for the purposes of an administrative or judicial procedure"@en .



###  http://purl.oclc.org/NET/ldr/ns#mirror

:mirror rdf:type :Distribution ,
                 owl:NamedIndividual ;
        
        rdfs:comment "The action of mirroring any piece of Linked Data"@en .



###  http://purl.oclc.org/NET/ldr/ns#nationalSecurity

:nationalSecurity rdf:type :CopyrightException ,
                           owl:NamedIndividual ;
                  
                  rdfs:comment "if the action is carried out in the interests of public security"@en .



###  http://purl.oclc.org/NET/ldr/ns#publicCommunication

:publicCommunication rdf:type :PublicCommunication ,
                              owl:NamedIndividual ;
                     
                     rdfs:comment "General right of public communication"@en .



###  http://purl.oclc.org/NET/ldr/ns#publishDatabase

:publishDatabase rdf:type :Reutilization ,
                          owl:NamedIndividual ;
                 
                 rdfs:comment "Make available a database in internet or by other means"@en .



###  http://purl.oclc.org/NET/ldr/ns#reasonWith

:reasonWith rdf:type :Access ,
                     owl:NamedIndividual ;
            
            rdfs:comment "Accesing Linked Data with the purpose of reasoning, through an specialized protocol (e.g. OWLLink) or not"@en .



###  http://purl.oclc.org/NET/ldr/ns#rebaseURIs

:rebaseURIs rdf:type :Derivation ,
                     owl:NamedIndividual ;
            
            rdfs:comment "Partially change the URI systematically rebasing the entities"@en .



###  http://purl.oclc.org/NET/ldr/ns#reificate

:reificate rdf:type :Derivation ,
                    owl:NamedIndividual ;
           
           rdfs:comment "Reificate an RDF statement or a set thereof"@en .



###  http://purl.oclc.org/NET/ldr/ns#rent

:rent rdf:type :Distribution ,
               owl:NamedIndividual ;
      
      rdfs:comment "Renting a copy of the work"@en .



###  http://purl.oclc.org/NET/ldr/ns#reproduction

:reproduction rdf:type :Reproduction ,
                       owl:NamedIndividual ;
              
              rdfs:comment "General right of public reproduction"@en .



###  http://purl.oclc.org/NET/ldr/ns#research

:research rdf:type :CopyrightException ,
                   owl:NamedIndividual ;
          
          rdfs:comment "illustration for teaching or scientific research, provided the source, including the author's name, is acknowledged"@en .



###  http://purl.oclc.org/NET/ldr/ns#reutilization

:reutilization rdf:type :Reutilization ,
                        owl:NamedIndividual ;
               
               rdfs:comment "General right of re-utilization"@en .



###  http://purl.oclc.org/NET/ldr/ns#sell

:sell rdf:type :Distribution ,
               owl:NamedIndividual ;
      
      rdfs:comment "Selling a copy of the work"@en .



###  http://purl.oclc.org/NET/ldr/ns#sellAccess

:sellAccess rdf:type :Distribution ,
                     owl:NamedIndividual ;
            
            rdfs:comment "Offering for meny the access to a copy of the work"@en .



###  http://purl.oclc.org/NET/ldr/ns#transcodeWork

:transcodeWork rdf:type :Derivation ,
                        owl:NamedIndividual ;
               
               skos:example "Having permission to publish a dataset as NTRIPLES, does not entitle the grantee the act of publishing the dataset as Turtle"@en ;
               
               rdfs:comment "Transcoding the work"@en .



###  http://purl.oclc.org/NET/ldr/ns#translateWork

:translateWork rdf:type :Derivation ,
                        owl:NamedIndividual ;
               
               skos:example "Having permission to publish a dataset, does not entitle the grantee the act of publishing a tanslated version of it"@en ;
               
               rdfs:comment "Translating the work"@en .



###  http://purl.org/NET/rdflicense/cc-zero1.0

<http://purl.org/NET/rdflicense/cc-zero1.0> rdf:type :FamousDataLicense ,
                                                     owl:NamedIndividual ;
                                            
                                            rdfs:label "CC0"@en ;
                                            
                                            rdfs:comment "Creative Commons public domain waiver"@en .



###  http://purl.org/NET/rdflicense/odbc-by1.0

<http://purl.org/NET/rdflicense/odbc-by1.0> rdf:type :FamousDataLicense ,
                                                     owl:NamedIndividual ;
                                            
                                            rdfs:label "Open Data Commons Attribution"@en ;
                                            
                                            rdfs:comment "Attribution for data/databases"@en .



###  http://purl.org/NET/rdflicense/odbc-pddl1.0

<http://purl.org/NET/rdflicense/odbc-pddl1.0> rdf:type :FamousDataLicense ,
                                                       owl:NamedIndividual ;
                                              
                                              rdfs:label "ODC Public Domain Dedication and Licence (PDDL)"@en ;
                                              
                                              rdfs:comment "Public Domain for data/databases"@en .



###  http://purl.org/NET/rdflicense/odbl1.0

<http://purl.org/NET/rdflicense/odbl1.0> rdf:type :FamousDataLicense ,
                                                  owl:NamedIndividual ;
                                         
                                         rdfs:label "ODC Open Database License"@en ;
                                         
                                         rdfs:comment "Attribution Share-Alike for data/databases"@en .



###  http://www.nationalarchives.gov.uk/doc/open-government-licence/version/2/

<http://www.nationalarchives.gov.uk/doc/open-government-licence/version/2/> rdf:type :FamousDataLicense ,
                                                                                     owl:NamedIndividual ;
                                                                            
                                                                            rdfs:label "UK Open Government License"@en ,
                                                                                       "UK Open Government License for public sector information"@en .





#################################################################
#
#    Annotations
#
#################################################################


owl:topObjectProperty rdfs:comment "hasIssuer"@en .



:RightsObject owl:deprecated "true"^^xsd:boolean ;
              
              rdfs:comment "Deprecated in favour of ODRL"@en ,
                           "Object over which a right is execised"@en ;
              
              skos:exactMatch odrl:Asset .



:Agent owl:deprecated "true"^^xsd:boolean ;
       
       rdfs:comment "Agent related to a Linked Data resource" ,
                    "Deprecated in favour of the ODRL term"@en ;
       
       skos:exactMatch odrl:Party ,
                       foaf:Agent .




###  Generated by the OWL API (version 3.4.2) http://owlapi.sourceforge.net

